theories/case_studies/multiuser_kvs/kvs_main_spec.v
@@ -67,7 +67,6 @@ Section KVS_main_spec.
       na_inv cerise_nais Nassert (assert_inv b_assert e_assert a_flag) ∗
       na_inv cerise_nais Nswitcher switcher_inv ∗
       na_inv cerise_nais Nkvs kvs_inv ∗
-      na_inv cerise_nais (Nkvs_user.@KVS_USER_KEY_MAIN) (logical_user_kvs_inv KVS_USER_KEY_MAIN) ∗
 
       inv (export_table_PCCN Nkvs_exp_tbl) (b_kvs_exp_tbl ↦ₐ WCap RX Global KVS_pcc_b KVS_pcc_e KVS_pcc_b) ∗
       inv (export_table_CGPN Nkvs_exp_tbl) ((b_kvs_exp_tbl ^+ 1)%a ↦ₐ WCap RW Global KVS_cgp_b KVS_cgp_e KVS_cgp_b) ∗
@@ -88,9 +87,10 @@ Section KVS_main_spec.
       [[ cgp_b , cgp_e ]] ↦ₐ [[ (kvs_main_data) ]] ∗
       [[ static_sealed_b , static_sealed_e ]] ↦ₐ [[ kvs_main_static_sealed KVS_USER_KEY_MAIN ]] ∗
 
+      logical_user_kvs_inv KVS_USER_KEY_MAIN ∗
       (KVS_USER_KEY_MAIN, 1) ↦(KVS) ⊥ ∗
-      world_interp W0 B ∗
 
+      world_interp W0 B ∗
       interp_continuation cstk Ws Cs ∗
       cstack_frag cstk ∗
 
@@ -105,12 +105,12 @@ Section KVS_main_spec.
                Hstatic_sealed_contiguous Hcgp_contiguous Himports_contiguous Hframe_match
             )
       "(#Hassert & #Hswitcher
-      & #Hkvs & #Hkvs_user
+      & #Hkvs
       & #Hkvs_exp_tbl_pcc & #Hkvs_exp_tbl_cgp & #Hkvs_exp_tbl_addOrUpdate & #Hkvs_exp_tbl_read
       & Hna
       & HPC & Hcgp & Hcsp & Hrmap
       & Himports_main & Hcode_main & Hcgp_main & Hstatic_sealed_main
-      & Hkvs_1
+      & HLUKVS & Hkvs_1
       & Hworld_B
       & HK & Hcstk_frag
       & #Hinterp_W0_B_f
@@ -316,12 +316,13 @@ Section KVS_main_spec.
 
     (* Use spec addOrUpdate known *)
     iApply (KVS_add_spec
-      with "[- $Hkvs $Hkvs_user $Hna $HPC $Hcgp $Hcra $ Hca0 $Hca1 $Hca2 $Hctp $Hct1 $Hct2 $Hcnull $Hstatic_sealed_b $Hkvs_1]")
+      with "[- $Hkvs $Hna $HPC $Hcgp $Hcra $ Hca0 $Hca1 $Hca2 $Hctp $Hct1 $Hct2 $Hcnull
+      $Hstatic_sealed_b $HLUKVS $Hkvs_1]")
     ; auto.
     { rewrite /is_uint16 /UINT16_MIN /UINT16_MAX; lia. }
     iNext;
       iIntros "(Hna & HPC & [% Hcgp] & [% Hcra] & Hca1 & [% Hca2]
-                    & [% Hctp] & [% Hct1] & [% Hct2] & [% Hcnull] & Hstatic_sealed_b & Hres)".
+                    & [% Hctp] & [% Hct1] & [% Hct2] & [% Hcnull] & Hstatic_sealed_b & HLUKVS & Hres)".
     iDestruct (big_sepM_sep with "Hrmap") as "[Hrmap _]".
 
     iInsertList "Hrmap" [ctp;ct1;ct2;cnull;ca2;ca3;ca4;ca5;ct0].
@@ -647,12 +648,13 @@ Section KVS_main_spec.
 
     (* Use spec readOrUpdate known *)
     iApply (KVS_read_spec_in
-      with "[- $Hkvs $Hkvs_user $Hna $HPC $Hcgp $Hcra $Hca0 $Hca1 $Hct1 $Hct2 $Hctp $Hcnull $Hstatic_sealed_b $Hkvs_1]")
+      with "[- $Hkvs $Hna $HPC $Hcgp $Hcra $Hca0 $Hca1 $Hct1 $Hct2 $Hctp $Hcnull
+            $Hstatic_sealed_b $HLUKVS $Hkvs_1]")
     ; auto.
     { rewrite /is_uint16 /UINT16_MIN /UINT16_MAX; lia. }
     iNext;
       iIntros "(Hna & HPC & [% Hcgp] & [% Hcra] & Hca0 & Hca1
-                & [% Hct1] & [% Hct2] & [% Hctp] & [% Hcnull] & Hstatic_sealed_b & Hkvs_1)".
+                & [% Hct1] & [% Hct2] & [% Hctp] & [% Hcnull] & Hstatic_sealed_b & HLUKVS & Hkvs_1)".
     iDestruct (big_sepM_sep with "Hrmap") as "[Hrmap _]".
 
     iInsertList "Hrmap" [ct1;ct2;ctp;cnull;ca2;ca3;ca4;ca5;ct0].
