theories/case_studies/multiuser_kvs/kvs_spec_read.v
@@ -243,13 +243,11 @@ Section KVS_spec_read.
     let fkey := (kvs_full_key user_key nkey) in
 
     ↑Nkvs ⊆ E ->
-    ↑Nkvs_user.@user_key ⊆ E ->
 
     is_uint16 nkey ->
     withinBounds user_key_addr (user_key_addr ^+ 1)%a user_key_addr = true ->
 
     ( na_inv cerise_nais Nkvs kvs_inv ∗
-      na_inv cerise_nais (Nkvs_user.@user_key) (logical_user_kvs_inv user_key) ∗
       na_own cerise_nais E ∗
 
       (* initial register file *)
@@ -265,6 +263,7 @@ Section KVS_spec_read.
 
       user_key_addr ↦ₐ WInt user_key ∗
 
+      ▷ logical_user_kvs_inv user_key ∗
       ▷ (user_key, nkey) ↦(KVS) w ∗
 
       ▷ (na_own cerise_nais E ∗
@@ -280,6 +279,7 @@ Section KVS_spec_read.
 
          user_key_addr ↦ₐ WInt user_key ∗
 
+         logical_user_kvs_inv user_key ∗
          (user_key, nkey) ↦(KVS) w
 
          -∗ WP Seq (Instr Executable) {{ v, ⌜v = HaltedV⌝ → na_own cerise_nais ⊤ }}
@@ -287,21 +287,22 @@ Section KVS_spec_read.
       ⊢ WP Seq (Instr Executable) {{ v, ⌜v = HaltedV⌝ → na_own cerise_nais ⊤ }})%I.
   Proof.
     intros fkey.
-    iIntros (Hnkvs_E Hnkvs_user_E His_uint16_nkey Hbounds_a_user_key)
-      "(#Hkvs_inv & #Hkvs_user_inv & Hna & HPC & Hcgp & Hcra & Hca0 & Hca1 & Hctp & Hct1 & Hct2 & Hcnull
-      & Ha_user_key & >Hk & Hpost)".
-    iMod (na_inv_acc with "Hkvs_user_inv Hna")
-      as "( (%ukvs & >Hukvs_auth & (%m & Hm & >%Hsync)) & Hna & Hkvs_user_inv_close)"; eauto.
+    iIntros (Hnkvs_E His_uint16_nkey Hbounds_a_user_key)
+      "(#Hkvs_inv & Hna & HPC & Hcgp & Hcra & Hca0 & Hca1 & Hctp & Hct1 & Hct2 & Hcnull
+      & Ha_user_key & (%ukvs & >Hukvs_auth & (%m & Hm & >%Hsync)) & >Hk & Hpost)".
 
     iDestruct (kvs_user_kvs_valid with "Hukvs_auth Hk") as "%Hk".
     opose proof (kvs_synced_logical_user_kvs_Some _ _ _ _ _ Hk) as Hm_kvs; eauto.
 
-    iApply (KVS_read_spec_in_layer_2 with "[- $HPC]"); last iFrame "∗#"; eauto.
-    { pose proof Nkvs_namespaces_disjoint as (?&?&?&?&?&?); solve_ndisj. }
-    iNext; iIntros "(Hna & HPC & Hcgp & Hcra & Hca0 & Hca1 & Hctp & Hct1 & Hct2 & Hcnull
-              & Ha_user_key & Hm)".
+    iApply (KVS_read_spec_in_layer_2
+             with "[- $Hkvs_inv $Hna
+                    $HPC $Hcgp $Hcra $Hca0 $Hca1 $Hctp $Hct1 $Hct2 $Hcnull
+                    $Ha_user_key $Hm]"); eauto.
+    iNext; iIntros "(Hna
+                    & HPC & Hcgp & Hcra & Hca0 & Hca1 & Hctp & Hct1 & Hct2 & Hcnull
+                    & Ha_user_key & Hm)".
 
-    iMod ("Hkvs_user_inv_close" with "[$Hna $Hukvs_auth $Hm]") as "Hna" ; auto.
+    iAssert (logical_user_kvs_inv user_key)%I with "[$Hm $Hukvs_auth]" as "Hlukvs"; auto.
 
     iApply "Hpost"; iFrame; done.
   Qed.
@@ -545,13 +546,11 @@ Section KVS_spec_read.
     :
 
     ↑Nkvs ⊆ E ->
-    ↑Nkvs_user.@user_key ⊆ E ->
 
     is_uint16 nkey ->
     withinBounds user_key_addr (user_key_addr ^+ 1)%a user_key_addr = true ->
 
     ( na_inv cerise_nais Nkvs kvs_inv ∗
-      na_inv cerise_nais (Nkvs_user.@user_key) (logical_user_kvs_inv user_key) ∗
       na_own cerise_nais E ∗
 
       (* initial register file *)
@@ -567,6 +566,7 @@ Section KVS_spec_read.
 
       user_key_addr ↦ₐ WInt user_key ∗
 
+      ▷ logical_user_kvs_inv user_key ∗
       ▷ (user_key, nkey) ↦(KVS) ⊥ ∗
 
       ▷ (na_own cerise_nais E ∗
@@ -579,27 +579,32 @@ Section KVS_spec_read.
          ct2 ↦ᵣ - ∗ (* scratch *)
          ctp ↦ᵣ - ∗ (* scratch *)
          cnull ↦ᵣ - ∗
+
          user_key_addr ↦ₐ WInt user_key ∗
+
+         logical_user_kvs_inv user_key ∗
          (user_key, nkey) ↦(KVS) ⊥
+
          -∗ WP Seq (Instr Executable) {{ v, ⌜v = HaltedV⌝ → na_own cerise_nais ⊤ }}
         )
       ⊢ WP Seq (Instr Executable) {{ v, ⌜v = HaltedV⌝ → na_own cerise_nais ⊤ }})%I.
   Proof.
-    iIntros (Hnkvs_E Hnkvs_user_E His_uint16_nkey Hbounds_a_user_key)
-      "(#Hkvs_inv & #Hkvs_user_inv & Hna & HPC & Hcgp & Hcra & Hca0 & Hca1 & Hctp & Hct1 & Hct2 & Hcnull
-      & Ha_user_key & >Hk & Hpost)".
-    iMod (na_inv_acc with "Hkvs_user_inv Hna")
-      as "( (%ukvs & >Hukvs_auth & (%m & Hm & >%Hsync)) & Hna & Hkvs_user_inv_close)"; eauto.
+    iIntros (Hnkvs_E His_uint16_nkey Hbounds_a_user_key)
+      "(#Hkvs_inv & Hna & HPC & Hcgp & Hcra & Hca0 & Hca1 & Hctp & Hct1 & Hct2 & Hcnull
+      & Ha_user_key & (%ukvs & >Hukvs_auth & (%m & Hm & >%Hsync)) & >Hk & Hpost)".
 
     iDestruct (kvs_user_kvs_valid with "Hukvs_auth Hk") as "%Hk".
     opose proof (kvs_synced_logical_user_kvs_None _ _ _ _ Hk) as Hm_kvs; eauto.
 
-    iApply (KVS_read_spec_notin_layer_2 with "[- $HPC]"); last iFrame "∗#"; eauto.
-    { pose proof Nkvs_namespaces_disjoint as (?&?&?&?&?&?); solve_ndisj. }
-    iNext; iIntros "(Hna & HPC & Hcgp & Hcra & Hca0 & Hca1 & Hctp & Hct1 & Hct2 & Hcnull
-              & Ha_user_key & Hm)".
+    iApply (KVS_read_spec_notin_layer_2
+             with "[- $Hkvs_inv $Hna
+                    $HPC $Hcgp $Hcra $Hca0 $Hca1 $Hctp $Hct1 $Hct2 $Hcnull
+                    $Ha_user_key $Hm]"); eauto.
+    iNext; iIntros "(Hna
+                    & HPC & Hcgp & Hcra & Hca0 & Hca1 & Hctp & Hct1 & Hct2 & Hcnull
+                    & Ha_user_key & Hm)".
 
-    iMod ("Hkvs_user_inv_close" with "[$Hna $Hukvs_auth $Hm]") as "Hna" ; auto.
+    iAssert (logical_user_kvs_inv user_key)%I with "[$Hm $Hukvs_auth]" as "Hlukvs"; auto.
 
     iApply "Hpost"; iFrame; done.
   Qed.
